adding IndexedTypesAgain module

DepCopland2.v
@@ -9,6 +9,12 @@ Module IndexedCopland.
     | BB : place
     | CC : place.
 
+   (* decidablility *)
+   Definition eq_place_dec: forall x y:place, {x=y}+{x<>y}.
+   Proof.
+   repeat decide equality.
+   Defined.
+
     (* The class is if the information is sensitive. Red means sensitive *)
     Inductive class : Type :=
     | red : class
@@ -22,83 +28,276 @@ Module IndexedCopland.
 
     (* Evidence structure indexed on the place. 
        This means place is captured with evidence *)
+       (* the place here is where we want the measurement to be taken *)
     Inductive evidence : place -> Type :=
     | EBlob : forall p, class -> evidence p
     | EHash : forall p, evidence p
-    | EPrivKey : forall p, evidence p
-    | EPubKey : forall p, evidence p
-    | ESessKey : forall p, nat -> evidence p
     | ECrypt : forall p q, evidence q -> place -> evidence p
     | ESig : forall p q, evidence q -> place -> evidence p
     | ESeq : forall p q r, evidence p -> evidence q -> evidence r
-    | EPar : forall p q r, evidence p -> evidence q -> evidence r
-    | EAt : forall q, place -> evidence q -> evidence q.
+    | EPar : forall p q r, evidence p -> evidence q -> evidence r.
+
+
+    Compute (ECrypt AA (EHash AA) AA). 
+
+    (*
+    BB = place to do encrypting 
+    CC = place blob is encrypted for 
+         only CC will be able to decrypt the blob  
+    *)
+    Compute (ECrypt BB (EBlob AA red) CC).
+    (* evidence BB *) 
+
+    Compute (ECrypt CC (EBlob AA red) CC).
 
     (* The privacy policy is a mapping from evidence to proposition *)
-    Fixpoint privPolicy p (e:evidence p): Prop :=
-        match e with
-        | EHash _ => True
-        | EBlob _ red => False
-        | EBlob _ green => True
-        | EPrivKey _ => False
-        | EPubKey _ => True
-        | ESessKey _ _ => False
-        | ESig _ e' _ => privPolicy e'
-        | ECrypt _ _ _ => True
-        | ESeq _ l r => (privPolicy l) /\ (privPolicy r)
-        | EPar _ l r => (privPolicy l) /\ (privPolicy r)
-        | EAt _ e' => privPolicy e'
+    Fixpoint privPolicy tp (ap:place) (e:evidence tp): Prop :=
+        match ap, e with
+        | _ , EHash _ => True
+        | _ , EBlob _ red => False
+        | _ , EBlob _ green => True
+        | ap, ESig _ e' _ => privPolicy ap e'
+        | ap, ECrypt p e' tp => if eq_place_dec ap tp then privPolicy ap e' else True
+        | _ , ESeq _ l r => (privPolicy ap l) /\ (privPolicy ap r)
+        | _ , EPar _ l r => (privPolicy ap l) /\ (privPolicy ap r)
         end.
 
-    (* terms are indexed on the evidence they produce *)
-    Inductive term p : (evidence p) -> Type :=
-    | TMeas : forall e, term e
-    | THash : forall e, term e -> privPolicy (EHash p) -> term (EHash p)
-    | TCrypt :
-        forall e q, term e -> privPolicy (ECrypt p e q) -> term (ECrypt p e q)
-    | TSig :
-        forall e q, term e -> privPolicy (ESig p e q) -> term (ESig p e q)
-    | TSeq : forall e f,
-        term e -> privPolicy e -> term f -> privPolicy f -> term (ESeq p e f)
-    | TPar : forall e f,
-        term e -> privPolicy e -> term f -> privPolicy f -> term (EPar p e f)
-    | TAt : forall p' e, 
-        term e -> privPolicy e -> term (EAt p' e).
+   Compute privPolicy CC (ECrypt BB (EBlob AA red) CC).
+   Compute privPolicy AA (ECrypt BB (EBlob AA red) CC). 
+        
+   Fixpoint privPolicy' tp (ap:place) (e:evidence tp): Prop :=
+      match ap, e with
+         | _ , EHash _ => True
+         | _ , EBlob _ red => False
+         | _ , EBlob _ green => True
+         | ap, ESig _ e' _ => privPolicy' ap e'
+         | ap, ECrypt _ e' tp => match e' with 
+                                 | EBlob p red => if eq_place_dec ap tp then False else True 
+                                 | _ => privPolicy' ap e'
+                                 end   
+         | _ , ESeq _ l r => (privPolicy' ap l) /\ (privPolicy' ap r)
+         | _ , EPar _ l r => (privPolicy' ap l) /\ (privPolicy' ap r)
+      end.
 
-    Lemma l1: forall p, privPolicy (EBlob p green). unfold privPolicy; auto. Qed.
-    Lemma l2: forall p q, privPolicy (ECrypt q (EBlob p red) p). unfold privPolicy; auto. Qed.
-    Lemma l3: forall p, privPolicy (EHash p). unfold privPolicy; auto. Qed.
-    Lemma l4: forall p, privPolicy (EAt p (EBlob p green)). unfold privPolicy; auto. Qed.
+      Compute privPolicy' CC (ECrypt BB (EBlob AA red) CC).
+      Compute privPolicy' AA (ECrypt BB (EBlob AA red) CC). 
+
+
+    (* terms are indexed on the evidence they produce *)
+    Inductive term p:(evidence p) -> Type :=
+    | TMeas : forall e, term e
+    | THash : forall ap e, term e -> privPolicy ap (EHash p) -> term (EHash p)
+    | TSig :
+         forall ap e q, term e -> privPolicy ap (ESig p e q) -> term (ESig p e q)
+    | TCrypt :
+        forall ap e q, term e -> privPolicy ap (ECrypt p e q) -> term (ECrypt p e q)
+    | TSeq : forall ap e f,
+        term e -> privPolicy ap e -> term f -> privPolicy ap f -> term (ESeq p e f)
+    | TPar : forall ap e f,
+        term e -> privPolicy ap e -> term f -> privPolicy ap f -> term (EPar p e f).
+
+
+    Lemma l1: forall ap p, privPolicy ap (EBlob p green). unfold privPolicy; auto. Qed.
+
+    Lemma l2_green: forall ap p q, privPolicy ap (ECrypt q (EBlob p green) p). unfold privPolicy. intros. destruct eq_place_dec. auto. auto. Qed.
+    (* this proof should only work with the prerequisite that ap <> p  *)
+    Lemma l2_red: forall ap p q, ap <> p -> privPolicy ap (ECrypt q (EBlob p red) p). intros.   
+    unfold privPolicy; intros; destruct eq_place_dec; auto. Qed.
+       
+       (* BB is the appraiser's place. CC is the place the target should encrypt from. *)
+    Compute TCrypt BB CC (TMeas (EBlob AA red)). 
+       (* : privPolicy BB (ECrypt AA (EBlob AA red) CC) ->
+          term (ECrypt AA (EBlob AA red) CC) *)
+
+    Lemma place_neq_AABB : AA <> BB. 
+    Proof. unfold not. intros. discriminate.
+    Qed.          
+   
+    Lemma place_neq_AACC : AA <> CC. 
+    Proof. unfold not. intros. discriminate.
+    Qed.  
+
+    Compute TCrypt AA CC (TMeas (EBlob BB red)) (l2_red BB place_neq_AACC).
+    (* term (ECrypt BB (EBlob BB red) CC)*)
+
+   Compute ECrypt BB (EBlob AA red) CC.
+   (* evidence BB *)
+   Compute TCrypt BB CC (TMeas (EBlob AA red)).
+   (* fun x : privPolicy BB (ECrypt AA (EBlob AA red) CC) =>
+       TCrypt BB CC (TMeas (EBlob AA red)) x
+     : privPolicy BB (ECrypt AA (EBlob AA red) CC) ->
+       term (ECrypt AA (EBlob AA red) CC) *) 
+   
+   
+
+    Lemma l3: forall ap p, privPolicy ap (EHash p). unfold privPolicy; auto. Qed.
     
     (* this lemma is written to include all pieces of evidence *)
-    Lemma l5: forall (p:place) (e:evidence p), privPolicy e = True -> term e. Proof. induction e; intros; apply TMeas. Qed.
+    Lemma l5: forall ap (p:place) (e:evidence p), privPolicy ap e = True -> term e. Proof. induction e; intros; apply TMeas. Qed.
 
     (* to write a term, you pass the TERM and a PROOF that the 
        term satisfies the privacy policy. *)
     Compute TMeas (EBlob AA green).
     Compute TMeas (EBlob AA red).
+    Compute TMeas (ECrypt BB (EBlob AA red) CC).
     Compute THash (TMeas (EBlob AA red)).
+    Compute THash (TMeas (EBlob AA red)) (l3 BB AA ).
 
-    (* something about l5 doesn't work right *)
-    (* Compute THash (TMeas (EBlob AA red)) (l5 (EHash AA) AA). *)
-    Compute THash (TMeas (EBlob AA red)) (l3 AA ).
-    Compute TCrypt (TMeas (EBlob AA red)) (l2 AA AA).
-    Compute TSig AA (TMeas (EBlob AA green)) (l1 AA).
+
+
+    (* Compute TSig AA AA (TMeas (EBlob AA green)) (l1 AA).
     Compute TSeq (TSig BB (TMeas (EBlob BB green)) (l1 BB)) (l1 BB)
                  (TCrypt (TMeas (EBlob BB red)) (l2 BB BB)) (l2 BB BB).
     Compute TPar (TSig BB (TMeas (EBlob BB green)) (l1 BB)) (l1 BB)
-                 (TCrypt (TMeas (EBlob BB red)) (l2 BB BB)) (l2 BB BB).
-    Compute TAt BB (TMeas (EBlob AA green)) (l4 BB).
+                 (TCrypt (TMeas (EBlob BB red)) (l2 BB BB)) (l2 BB BB). *)
 
-    (* because the privacy policy is already included in the term structure... 
-       how do we generate all terms that are true?? *)
-    Definition selectDep p (e:evidence p) := {t:term e | privPolicy e}.
-    
-    Compute selectDep (EBlob BB red).
-    Compute selectDep (EAt BB (EBlob AA green)).
-    Compute selectDep (ECrypt BB (EBlob BB red) BB). 
 
 End IndexedCopland. 
+
+Module IndexedTypesAgain. 
+
+   (* The place is where we want the measurement from *)
+   Inductive place : Type :=
+   | AA : place
+   | BB : place
+   | CC : place
+   | DD : place 
+   | EE : place .
+
+   (* decidablility *)
+   Definition eq_place_dec: forall x y:place, {x=y}+{x<>y}.
+   Proof.
+   repeat decide equality.
+   Defined.
+
+    (* The class is if the information is sensitive. Red means sensitive *)
+   Inductive class : Type :=
+   | red : class
+   | green : class.
+
+    (* decidablility *)
+    Definition eq_class_dec: forall x y:class, {x=y}+{x<>y}.
+    Proof.
+    repeat decide equality.
+    Defined.
+
+   (* here, the structure of evidence is a Set 
+       https://ku-sldg.github.io/copland/resources/coplandcoq/html/Copland.Term.html *)
+   (* This structure has type: evidence _ where _ is the place where evidnece is gathered*)
+   Inductive evidence : place -> Type :=
+   | EBlob : forall p, class -> evidence p
+   | EHash : forall p, evidence p
+   | ECrypt : forall p q, evidence q -> place -> evidence p
+   | ESig : forall p q, evidence q -> place -> evidence p
+   | ESeq : forall p q r, evidence p -> evidence q -> evidence r
+   | EPar : forall p q r, evidence p -> evidence q -> evidence r.
+
+   Compute (ESeq AA (EBlob BB green) (EBlob CC red)).
+   (* evidence AA *)
+   Compute (ECrypt AA (EBlob BB green) CC).
+   (* evidence AA *) 
+
+   (* where do I pass the proof argument here? *)
+   Lemma eqAA : AA = AA. reflexivity. Qed.  
+   Compute eq_place_dec AA AA. 
+
+   Definition a1 : {AA = AA} + {AA <> AA} := left _ eqAA .
+   Check a1. 
+   
+   Lemma less37: 3<7. Proof. auto. Qed.
+   Definition v3: {3<7}+{~(3<7)} := left _ less37.
+   Check left _ less37. 
+
+    Fixpoint privPolicy (ap:place) tp (e:evidence tp): Prop :=
+      match e with
+      | EHash _ => True
+      | EBlob _ red => False
+      | EBlob _ green => True
+      | ESig _ e' _ => privPolicy ap e'
+      | ECrypt _ e' tp => if eq_place_dec ap tp then privPolicy ap e' else True
+      | ESeq _ l r => (privPolicy ap l) /\ (privPolicy ap r)
+      | EPar _ l r => (privPolicy ap l) /\ (privPolicy ap r)
+      end.
+
+   (* Checking to make sure the privacy policy is written correctly for ECrypt. 
+      The appraiser's place should should not match the place where encryption is 
+      occuring if the blob is red  *)
+   Compute privPolicy CC (ECrypt AA (EBlob AA red) CC).
+   Compute privPolicy CC (ECrypt CC (EBlob CC red) AA).
+   Compute privPolicy CC (ECrypt AA (EBlob AA red) BB).
+   
+   (* This measuement type checks but would be impossible to write
+      with the way the type system works.
+      
+      For some reason, I can't figure out how to get the crypt 
+      measurement to have place CC. It is always the 
+      same place as AA *)
+   Compute privPolicy CC (ECrypt CC (EBlob AA red) BB).
+
+    (* Terms are indexed on the evidence they produce. First, they expect some measurement.
+       That is the first parameter that comes with `term e`. It may also expect the place that 
+       is asking for the measurment, ap.   *)
+    Inductive term p:(evidence p) -> Type :=
+    | TMeas : forall e, term e
+    | THash : forall ap e, term e -> privPolicy ap (EHash p) -> term (EHash p)
+    | TSig :
+         forall ap e q, term e -> privPolicy ap (ESig p e q) -> term (ESig p e q)
+    | TCrypt :
+        forall ap e q, term e -> privPolicy ap (ECrypt p e q) -> term (ECrypt p e q)
+    | TSeq : forall ap e f,
+        term e -> privPolicy ap e -> term f -> privPolicy ap f -> term (ESeq p e f)
+    | TPar : forall ap e f,
+        term e -> privPolicy ap e -> term f -> privPolicy ap f -> term (EPar p e f).
+
+   (* this returns some funky thing where we must provide a proof that the 
+      goal is satisfied. As input, we give it the apprasier's place, AA. The place 
+      where we want the encryption to occur, and the measurement.  *)
+   Compute TCrypt AA BB (TMeas (EBlob CC green)) . 
+   (* = fun x : privPolicy AA (ECrypt CC (EBlob CC green) BB) =>
+       TCrypt AA BB (TMeas (EBlob CC green)) x
+     : privPolicy AA (ECrypt CC (EBlob CC green) BB) ->
+       term (ECrypt CC (EBlob CC green) BB) *)
+
+   (* proof that any green measurement is acceptable *)
+   Lemma tmeas_green : forall p, privPolicy p (EBlob p green).
+   Proof. intros. simpl. auto. Qed.   
+
+   (* it shouldn't matter if ap = tp... the blob is green
+      the privacy policy for crypt must take into consideration 
+      - ap -- the appraiser's place 
+      - mp -- the measurement place 
+      - ep -- the evidence gathered place  *)
+   Lemma green_crypted: forall ap mp ep, privPolicy ap (ECrypt mp (EBlob mp green) ep).
+   Proof. intros. simpl. destruct eq_place_dec. auto. auto. Qed.
+   
+   Compute TCrypt AA BB (TMeas (EBlob CC green)) (green_crypted AA CC BB).
+   (*  = TCrypt AA BB (TMeas (EBlob CC green)) (green_crypted AA CC BB)
+       : term (ECrypt CC (EBlob CC green) BB) 
+       
+       This says that the green blob measured at place CC is encrypted with BB. *) 
+
+   (* A red measurement should be okay if the appraiser place is not the same as the 
+      encryption place (ep)*)
+   Lemma red_crypted: forall ap ep r, ap <> ep -> privPolicy ap (ECrypt r (EBlob r red) ep).
+   Proof.  intros. unfold privPolicy. destruct eq_place_dec. auto. auto. Qed.
+   
+   (* This proof is True. It has type AA <> CC *)
+   Lemma neqAACC : AA <> CC. unfold not; intros; discriminate. Qed.  
+   Check neqAACC. 
+
+   (* for some reason, all we need is ONE proof. We can reuse this proof no 
+      matter the places? *)
+   Compute TCrypt AA CC (TMeas (EBlob CC red)) (red_crypted AA neqAACC).
+   (* = TCrypt AA CC (TMeas (EBlob CC red)) (red_crypted AA neqAACC)
+      : term (ECrypt CC (EBlob CC red) CC)*)
+   Compute TCrypt AA BB (TMeas (EBlob CC red)) (red_crypted AA neqAACC).   
+   (* = TCrypt AA BB (TMeas (EBlob CC red)) (red_crypted AA neqAACC)
+     : term (ECrypt CC (EBlob CC red) BB)*)
+
+   (* BUT it does not work if the first two places match... which was the goal. *)
+   (* Compute TCrypt AA AA (TMeas (EBlob CC red)) (red_crypted AA neqAACC). *) 
+
+End IndexedTypesAgain. 
 
 Module SubCopland.
 
@@ -106,6 +305,18 @@ Inductive place : Type :=
 | AA : place
 | BB : place
 | CC : place.
+
+Fixpoint place_match (p1 p2: place) : Prop :=
+   match p1 with 
+   | AA => True
+   | CC => False 
+   | BB => True 
+   end. 
+
+Definition eq_place_dec: forall x y:place, {x=y}+{x<>y}.
+Proof.
+  repeat decide equality.
+Defined.
 
 Inductive class : Type :=
 | red : class
@@ -135,47 +346,62 @@ Defined.
 Inductive term : evidence -> Type :=
 | TMeas : forall e, term e
 | THash : forall e, term e -> term EHash
-| TCrypt : forall e p, term e -> term (ECrypt e p)
 | TSig : forall e p, term e -> term (ESig e p)
+| TCrypt : forall e p, term e -> term (ECrypt e p)
 | TSeq : forall e f, term e -> term f -> term (ESeq e f)
 | TPar : forall e f, term e -> term f -> term (EPar e f)
 | TAt : forall e p, term e -> term (EAt p e).
 
 Check TMeas (EBlob green).
 
-(* privacy policy mapping from evidence to Proposition *)
-(* we MUST define privacy policy over evidence bc we need to make 
-   sure the evidence doesn't evalute to expose sensitive information *)
-(* We include place in the privacy policy to  *)
-Fixpoint privPolicyProp (rp : place) (e:evidence): Prop :=
-    match rp, e with
-    | _ , EHash => True
-    | _ , EBlob red => False
-    | _ , EBlob green => True
-    | _ , ECrypt e p =>  match rp with 
-                           | p => privPolicyProp rp e
-                           (* | _ => True *)
-                           end
-    | _ , ESig e' _ => privPolicyProp rp e'
-    | _ , ESeq l r => and (privPolicyProp rp l) (privPolicyProp rp r)
-    | _ , EPar l r => and (privPolicyProp rp l) (privPolicyProp rp r)
-    | _ , EAt p e' => privPolicyProp rp e' 
+(* privacy policy mapping from evidence to Proposition 
+
+   we MUST define privacy policy over evidence bc we need to make 
+   sure the evidence doesn't evalute to expose sensitive information 
+
+   We include place in the privacy policy to make sure that if a red blob 
+   is encrypted, the appraiser cannot decrypt it. *)
+Fixpoint privPolicyProp (ap : place) (e:evidence): Prop :=
+    match e with
+    | EHash => True
+    | EBlob red => False
+    | EBlob green => True
+    | ECrypt e tp =>  if eq_place_dec ap tp then privPolicyProp ap e else True
+    | ESig e' _ => privPolicyProp ap e'
+    | ESeq l r => and (privPolicyProp ap l) (privPolicyProp ap r)
+    | EPar l r => and (privPolicyProp ap l) (privPolicyProp ap r)
+    | EAt p e' => privPolicyProp ap e' 
     end.
 
     Compute TMeas (ECrypt (EBlob green) AA).
     Compute privPolicyProp (AA) (ECrypt (EBlob green) AA).
+    (* = True
+     : Prop *)
     Compute privPolicyProp (AA) (ECrypt (EBlob red) AA).
+    (* = False
+     : Prop*)
     Compute privPolicyProp (BB) (ECrypt (EBlob green) AA).
+    (* = True
+     : Prop *)
+   Compute privPolicyProp (BB) (ECrypt (EBlob red) AA).
+   (* We can encrypt a RED blob as long as the place recieving cannot decrypt it
+   
+      = True 
+      : Prop 
+   *)
 
-    Definition privPolicyTProp p e (t:term e) := privPolicyProp p e.
+   (* this privacy policy takes in a place asking *)
+   Definition privPolicyTProp p e (t:term e) := privPolicyProp p e.
 
     (* This is our selection policy which creates a set of terms. 
        It builds the set based on privacy policy satisfaction.   *)
     Definition selectDep p e (_:term e) := {t:term e | privPolicyProp p e}.
+    
+    (* Definition selectDep e (_:term e) := {t:term e | privPolicyProp e}. *)
 
     Check selectDep. 
     (* selectDep
-       : forall e : evidence, term e -> Set*) 
+       : place -> forall e : evidence, term e -> Set*) 
     (* the return type of selectDep is a SET. *)
     
     
